@prefix : <http://sensorml.com/ont/eor/property/> .
@prefix owl: <http://www.w3.org/2002/07/owl#> .
@prefix rdf: <http://www.w3.org/1999/02/22-rdf-syntax-ns#> .
@prefix xml: <http://www.w3.org/XML/1998/namespace> .
@prefix xsd: <http://www.w3.org/2001/XMLSchema#> .
@prefix rdfs: <http://www.w3.org/2000/01/rdf-schema#> .
@base <http://sensorml.com/ont/eor/property> .

<http://sensorml.com/ont/eor/property> rdf:type owl:Ontology ;
                                    owl:imports <http://qudt.org/2.1/vocab/quantitykind> ,
                                                <http://www.w3.org/ns/ssn/systems/> ;
                                    <http://purl.org/dc/terms/creator> "OpenSensorHub Community" ;
                                    rdfs:label "SensorWeb Electro-Optical & Radar Properties Ontology" ;
                                    owl:versionInfo 1.0 .

#################################################################
#    Annotation properties
#################################################################

###  http://www.w3.org/2004/02/skos/core#narrower
<http://www.w3.org/2004/02/skos/core#narrower> rdf:type owl:AnnotationProperty .


###  http://www.w3.org/2004/02/skos/core#related
<http://www.w3.org/2004/02/skos/core#related> rdf:type owl:AnnotationProperty .


#################################################################
#    Individuals
#################################################################

###  http://sensorml.com/ont/eor/property/GroundSampleDistance
:GroundSampleDistance rdf:type owl:NamedIndividual ,
                           <http://qudt.org/vocab/quantitykind/Distance> ;
                  <http://www.w3.org/2004/02/skos/core#definition> "The Ground Sample Distance (GSD, or Ground Resolution) is the distance between pixel centers of a digital photo of the earth surface, taken from the air or space (such as an orthophoto), and measured on the ground. It is usually measured in meters or kilometers" .

###  http://sensorml.com/ont/eor/property/AlongTrackGSD
:AlongTrackGSD rdf:type owl:NamedIndividual ,
                           <http://qudt.org/vocab/quantitykind/Distance> ;
                  <http://www.w3.org/2004/02/skos/core#definition> "Ground sample distance of a satellite-borne sensor measured in the along-track direction, that is along the satellite ground track (i.e. the projection of the orbit on the earth surface)" .

###  http://sensorml.com/ont/eor/property/AcrossTrackGSD
:AcrossTrackGSD rdf:type owl:NamedIndividual ,
                           <http://qudt.org/vocab/quantitykind/Distance> ;
                  <http://www.w3.org/2004/02/skos/core#definition> "Ground sample distance of a satellite-borne sensor measured in the across-track direction, that is orthogonally to the satellite ground track (i.e. the projection of the orbit on the earth surface)" .





###  Generated by the OWL API (version 4.5.9.2019-02-01T07:24:44Z) https://github.com/owlcs/owlapi
