@prefix : <http://sensorml.com/ont/system_types/> .
@prefix owl: <http://www.w3.org/2002/07/owl#> .
@prefix rdf: <http://www.w3.org/1999/02/22-rdf-syntax-ns#> .
@prefix xml: <http://www.w3.org/XML/1998/namespace> .
@prefix xsd: <http://www.w3.org/2001/XMLSchema#> .
@prefix rdfs: <http://www.w3.org/2000/01/rdf-schema#> .
@base <http://sensorml.com/ont/core/system> .

<http://sensorml.com/ont/core/system> rdf:type owl:Ontology ;
                                       owl:imports <http://www.w3.org/ns/ssn/systems/> ;
                                       <http://purl.org/dc/terms/creator> "Alex Robin" ;
                                       rdfs:comment "Ontology of generic system and component types" ;
                                       rdfs:label "SensorWeb System Types Ontology" ;
                                       owl:versionInfo 1.0 .

#################################################################
#    Classes
#################################################################

###  http://sensorml.com/ont/core/system/ComputerModel
<http://sensorml.com/ont/core/system/ComputerModel> rdf:type owl:Class ;
                                                    rdfs:subClassOf <http://www.w3.org/ns/sosa/Sensor> ;
                                                    <http://www.w3.org/2004/02/skos/core#definition> """A computer model (or computer simulation) is designed to predict the behaviour or the outcome of a real-world or physical system. In the context of Sensor Web, it can also be seen as a type of (virtual) Sensor that estimates or forecasts the value of observed properties using some kind of software algorithm.

A computer model often takes real-world measurements as inputs and processes them further by applying a mathematical model such as the equations of various fields of physics. As such, it also a kind of DataProcessor.

Example of computer models are weather forecast models, flood models, Kalman filters, etc.""" .


###  http://sensorml.com/ont/core/system/DataProcessor
<http://sensorml.com/ont/core/system/DataProcessor> rdf:type owl:Class ;
                                                    rdfs:subClassOf <http://www.w3.org/ns/ssn/System> ;
                                                    rdfs:seeAlso <https://en.wikipedia.org/wiki/Information_processor> ;
                                                    <http://www.w3.org/2004/02/skos/core#definition> "A system component used to process digital data, such as an on-board computer." .


###  http://sensorml.com/ont/core/system/DataTransmitter
<http://sensorml.com/ont/core/system/DataTransmitter> rdf:type owl:Class ;
                                                      rdfs:subClassOf <http://www.w3.org/ns/ssn/System> ;
                                                      rdfs:seeAlso <https://en.wikipedia.org/wiki/Data_transmission> ;
                                                      <http://www.w3.org/2004/02/skos/core#definition> """A System component used to transmit and receive data over a point-to-point or point-to-multipoint communication channel.

In the context of the Sensor Web, its most relevant use is to transmit observation data produced by the System's Sensors and receive command data targeted at the System's Actuators.""" .


###  http://sensorml.com/ont/core/system/Detector
<http://sensorml.com/ont/core/system/Detector> rdf:type owl:Class ;
                                               rdfs:subClassOf <http://www.w3.org/ns/sosa/Sensor> ;
                                               <http://www.w3.org/2004/02/skos/core#definition> "A Detector is an atomic sensing element (often analog) that is sensitive to a single observable property. It is a fundamental part of any Sensor." .


###  http://sensorml.com/ont/core/system/DigitalSensor
<http://sensorml.com/ont/core/system/DigitalSensor> rdf:type owl:Class ;
                                                    rdfs:subClassOf <http://www.w3.org/ns/sosa/Sensor> ;
                                                    <http://www.w3.org/2004/02/skos/core#definition> "A Digital Sensor is a type of electronic, electro-mechanical or electro-chemical Sensor device composed of one or more Detectors and additional electronics, used jointly to compute and output a digital representation of each observed Property." .


###  http://sensorml.com/ont/core/system/HumanSensor
<http://sensorml.com/ont/core/system/HumanSensor> rdf:type owl:Class ;
                                                  rdfs:subClassOf <http://www.w3.org/ns/sosa/Sensor> ;
                                                  <http://www.w3.org/2004/02/skos/core#definition> "A human acting as a Sensor, for example in the context of a poll, a survey, an inspection, a review, or by simply reporting stimuli received by its sensory organs." .


###  http://sensorml.com/ont/core/system/SensorArray
<http://sensorml.com/ont/core/system/SensorArray> rdf:type owl:Class ;
                                                  rdfs:subClassOf <http://sensorml.com/ont/core/system/SensorSystem> ;
                                                  <http://www.w3.org/2004/02/skos/core#definition> """A Sensor Array is a group of identical (or almost identical) Sensors that are collectively used to homogeneously observe the same set of properties of one or more Features of Interest.

It is often used to observe a single sampled feature at different sampling locations, in which case the resulting data can often be represented as a coverage.""" .


###  http://sensorml.com/ont/core/system/SensorNetwork
<http://sensorml.com/ont/core/system/SensorNetwork> rdf:type owl:Class ;
                                                    rdfs:subClassOf <http://sensorml.com/ont/core/system/SensorSystem> ;
                                                    <http://www.w3.org/2004/02/skos/core#definition> "A Sensor Network is a group of spatially dispersed and dedicated Sensors collectively used for measuring properties of one or more Features of Interest and whose data is collected and organized in a common manner." .


###  http://sensorml.com/ont/core/system/SensorSystem
<http://sensorml.com/ont/core/system/SensorSystem> rdf:type owl:Class ;
                                                   rdfs:subClassOf <http://www.w3.org/ns/sosa/Sensor> ;
                                                   <http://www.w3.org/2004/02/skos/core#definition> "A (measurement) System that itself acts as a Sensor (i.e. has its own outputs) and composed of one or more Sensor and DataProcessor components." .


###  Generated by the OWL API (version 4.5.9.2019-02-01T07:24:44Z) https://github.com/owlcs/owlapi
